Tree_calculus/offcuts.v
@@ -1,0 +1,239 @@
+
+(* 
+Lemma star_opt_app_comb2:
+  forall M N, maxvar M = 0 -> occurs 0 N = true -> occurs 1 N = true -> 
+              star_opt (star_opt (app_comb M  N)) = k_op.
+Proof.
+  intros.
+  rewrite star_opt_app_comb1; auto.   
+  rewrite star_opt_occurs_true. 
+  2: simpl; rewrite H0; auto.
+  2: rewrite ! orb_false_r.
+  2: replace (match N with
+      | Ref 0 => subst k_op (Op Node)
+      | _ =>
+          App (App (Op Node) (App (Op Node) (star_opt N)))
+            (App k_op (subst (App node node) (Op Node)))
+      end)
+    with (App (App (Op Node) (App (Op Node) (star_opt N)))
+              (App k_op (subst (App node node) (Op Node)))).
+  all: cycle 1.
+  simpl. 
+  rewrite occurs_star_opt.
+  rewrite H1; auto. simpl. 
+  rewrite orb_true_r.   auto.
+  2: discriminate.
+  gen2_case H0 H1 N.
+  assert False.
+  gen2_case H0 H1 n; discriminate. omega. 
+  (* 1 *)
+  assert (match N with
+      | Ref 0 => subst k_op (Op Node)
+      | _ =>
+          App (App (Op Node) (App (Op Node) (star_opt N)))
+            (App k_op (subst (App node node) (Op Node)))
+          end =
+          App (App (Op Node) (App (Op Node) (star_opt N)))
+              (App k_op (subst (App node node) (Op Node)))).
+  gen2_case H0 H1 N.
+  assert False.
+  gen2_case H0 H1 n; discriminate. omega. 
+  rewrite star_opt_closed. 
+  2: cbv; auto.
+  rewrite star_opt_occurs_true. 
+  2: simpl; rewrite H0; auto.
+  2: rewrite ! orb_false_r.
+  2: rewrite H2.  
+  2: simpl; auto. 
+  all: cycle 1.
+rewrite occurs_star_opt.   
+rewrite H1.   simpl. rewrite orb_true_r. auto.
+discriminate.
+  rewrite star_opt_occurs_true. 
+  2: simpl; rewrite H0; auto.
+  2: rewrite ! orb_false_r.
+  2: rewrite H2.  
+  2: simpl; auto. 
+  all: cycle 1.
+rewrite occurs_star_opt.   
+rewrite H1.   simpl. rewrite orb_true_r. auto.
+discriminate.
+  rewrite star_opt_occurs_true. 
+  2: simpl; rewrite H0; auto.
+  2: rewrite ! orb_false_r.
+  2: rewrite H2.  
+  2: simpl; auto. 
+  all: cycle 1.
+rewrite occurs_star_opt.   
+rewrite H1.   simpl. rewrite orb_true_r. auto.
+discriminate.
+  rewrite star_opt_occurs_true. 
+  2: simpl; rewrite H0; auto.
+  2: rewrite ! orb_false_r.
+  2: rewrite H2.  
+  2: simpl; auto. 
+  all: cycle 1.
+rewrite occurs_star_opt.   
+rewrite H1. auto.    
+discriminate.
+rewrite star_opt_closed. 
+2: cbv; auto.
+rewrite star_opt_occurs_true.
+2: rewrite ! occurs_app. 
+2: rewrite ! occurs_op.
+2: rewrite occurs_star_opt. 
+2: rewrite ! occurs_app. 2: rewrite H1. 2: cbv; auto. 2: discriminate.
+rewrite star_opt_occurs_true.
+2: rewrite ! occurs_app. 
+2: rewrite ! occurs_op.
+2: rewrite occurs_star_opt. 
+2: rewrite ! occurs_app. 2: rewrite H1. 2: cbv; auto. 2: discriminate.
+
+
+
+simpl2: rewrite H2. cbv; auto. 2: discriminate. 
+  2: simpl; rewrite H0; auto.
+  2: rewrite ! orb_false_r.
+  2: rewrite H2.  
+  2: simpl; auto. 
+  all: cycle 1.
+rewrite occurs_star_opt.   
+rewrite H1.   simpl. rewrite orb_true_r. auto.
+discriminate.
+  rewrite star_opt_occurs_true. 
+  2: simpl; rewrite H0; auto.
+  2: rewrite ! orb_false_r.
+  2: rewrite H2.  
+  2: simpl; auto. 
+  all: cycle 1.
+rewrite occurs_star_opt.   
+rewrite H1.   simpl. rewrite orb_true_r. auto.
+discriminate.
+  rewrite star_opt_occurs_true. 
+  2: simpl; rewrite H0; auto.
+  2: rewrite ! orb_false_r.
+  2: rewrite H2.  
+  2: simpl; auto. 
+  all: cycle 1.
+rewrite occurs_star_opt.   
+rewrite H1.   simpl. rewrite orb_true_r. auto.
+discriminate.
+
+
+
+assert False.
+  gen2_case H0 H1 n; discriminate. omega. 
+
+
+  2: rewrite ! orb_false_r.
+
+
+
+  all: try discriminate.
+  rewrite H0.  rewrite occurs_closed. simpl. 
+  unfold eqnat in *.
+
+  2: congruence. 
+  rewrite star_opt_occurs_true. 
+  2: simpl; rewrite H0; auto. 2: congruence. 
+  rewrite star_opt_closed. 
+  2: cbv; auto.
+  rewrite star_opt_occurs_true. 
+  2: simpl; rewrite H0; auto. 2: congruence. 
+  rewrite star_opt_occurs_true. 
+  2: simpl; rewrite H0; auto. 2: congruence. 
+  rewrite (star_opt_closed  (App (Op Node) (App (Op Node) i_op))).
+  2: cbv; auto.
+  rewrite ! (star_opt_closed (Op Node)).
+  2: cbv; auto. auto. 
+Qed.
+
+
+(* 
+
+  Lemma star_opt_app_comb:
+  forall M1 N1 M2 N2, maxvar M1 = 0 -> maxvar M2 = 0 -> occurs 0 N1 = occurs 0 N2 ->
+                      star_opt (app_comb M1 N1) = star_opt (app_comb M2 N2) ->
+                      M1 = M2 /\ star_opt N1 = star_opt N2.
+Proof.
+  intros.
+  assert (occurs 0 N1 = false \/ occurs 0 N1 <> false) by decide equality.  
+  inversion H3.
+  (* 2 *) 
+rewrite ! star_opt_occurs_false in *. 
+inversion H2. split.  rewrite ! subst_rec_closed in H7. auto. omega. omega. congruence. 
+unfold app_comb; simpl.   rewrite H4 in *. rewrite <- H1. rewrite occurs_closed.
+auto. auto. congruence.
+unfold app_comb; simpl.   rewrite H4 in *. rewrite occurs_closed.
+auto. auto. congruence.
+(* 1 *)
+generalize H2; clear H2.  unfold app_comb. 
+  rewrite star_opt_occurs_true at 1.   
+  rewrite star_opt_occurs_true at 1.   
+  2: unfold_op; simpl.
+  2: gen_case H4 (occurs 0 N1). 2: congruence. 2: unfold_op; simpl.
+  2: gen_case H4 (occurs 0 N1). 2: congruence. 
+  rewrite star_opt_closed at 1. 2: simpl; auto. 
+  rewrite star_opt_occurs_true at 1.   
+  2: unfold_op; simpl.
+  2: gen_case H4 (occurs 0 N1). 2: congruence.
+  rewrite star_opt_occurs_true at 1.   
+  2: unfold_op; simpl.
+  2: gen_case H4 (occurs 0 N1). 2: congruence.
+  unfold star_opt at 2 3.
+  rewrite (star_opt_closed (App (Op Node) _)). 
+  2: cbv; auto.
+
+  intro. 
+assert(star_opt
+         (App (App (Op Node) (App (Op Node) i_op))
+              (App (App (Op Node) (App (Op Node) (App k_op N2))) (App k_op M2))) =
+        App
+         (App (Op Node)
+            (App (Op Node)
+               (App (App (Op Node) (App (Op Node) (App k_op (App k_op M1))))
+                  (App
+                     (App (Op Node)
+                        (App (Op Node)
+                           (App (App (Op Node) (App (Op Node) (star_opt (App k_op N1))))
+                              (App k_op (Op Node))))) (App k_op (Op Node))))))
+         (App k_op (App (Op Node) (App (Op Node) i_op))) )
+     by auto.   
+generalize H5; clear H2 H5.
+assert(occurs 0 N2 = true). gen2_case H4 H1 (occurs 0 N1). 
+rewrite star_opt_occurs_true at 1.   
+  rewrite star_opt_occurs_true at 1.   
+  2: unfold_op; simpl.
+  2:  rewrite H2; auto. 2:congruence. 2: unfold_op; simpl.
+  2: rewrite H2; auto. 2: congruence. 
+  rewrite star_opt_closed at 1. 2: simpl; auto. 
+  rewrite star_opt_occurs_true at 1.   
+  2: unfold_op; simpl.
+  2: auto.  2: congruence.
+  rewrite star_opt_occurs_true at 1.   
+  2: unfold_op; simpl.
+  2: auto. 2: congruence.
+  unfold star_opt at 2 3.
+  rewrite (star_opt_closed (App (Op Node) _)). 
+  2: cbv; auto.
+
+  intro. inversion H5; subst.
+  rewrite H2 in *.
+  assert(occurs 0 N1 = true) by (gen_case H4 (occurs 0 N1)). 
+  rewrite H6 in *. 
+  split; auto. 
+  clear - H2 H6 H8.
+  gen2_case H2 H8 N2. 
+  gen2_case H2 H8 n.
+  gen2_case H6 H8 N1. 
+  gen2_case H6 H8 n0.
+  all: try discriminate.   
+  gen2_case H6 H8 N1. 
+  gen2_case H6 H8 n.
+  gen2_case H2 H8 (occurs 0 t).
+all: try (inversion H8; fail).   
+all: try discriminate. 
+inversion H8; subst. auto. 
+Qed.
+ *) 
+ *)
